try to prove loop rule

theories/cf_lang/multi_post.v
@@ -3,7 +3,7 @@ From iris.proofmode Require Import coq_tactics reduction.
 From iris.proofmode Require Import tactics.
 From iris.algebra Require Import auth gmap.
 From iris.base_logic Require Export gen_heap.
-From iris.base_logic.lib Require Export proph_map.
+From iris.base_logic.lib Require Export proph_map invariants.
 From iris.program_logic Require Import atomic.
 From iris.program_logic Require Export weakestpre total_weakestpre.
 From iris.program_logic Require Import ectx_lifting total_ectx_lifting.
@@ -29,25 +29,27 @@ Section multi_post.
 
 Context `{!heapG Σ}.
 
-Definition multi_post (φn φb φc φr : sval -> iPropI Σ) v : iPropI Σ :=
+Definition multi_post (φn φb φc φr : val -> iPropI Σ) v : iPropI Σ :=
   match v with
-  | SVal _ => φn v
-  | SBreak _ => φb v
-  | SContinue => φc v
-  | SReturn _ => φr v
+  | SVal v => φn v
+  | SBreak v => φb v
+  | SContinue => φc $ LitV LitUnit
+  | SReturn v => φr v
   end.
 
-Definition top (v:sval) : iPropI Σ := bi_pure True.
-Definition bot (v:sval) : iPropI Σ := bi_pure False.
+Definition top (v:val) : iPropI Σ := bi_pure True.
+Definition bot (v:val) : iPropI Σ := bi_pure False.
 
-Notation "'WP' e @ s ; E {{ φn } } {{ φb } } {{ φc } } {{ φr } }" := 
-  (wp s E e%E (multi_post φn φb φc φr)) (at level 20, e, φn, φb, φc, φr at level 200).
+Notation "'WP' e {{ φn } } {{ φb } } {{ φc } } {{ φr } }" := 
+  (wp NotStuck ⊤ e%E (multi_post φn φb φc φr)) (at level 20, e, φn, φb, φc, φr at level 200).
 
+Notation "'{{' P } } e {{ φn } } {{ φb } } {{ φc } } {{ φr } }" :=
+  (uPred_persistently (P -∗ WP e {{ φn }} {{ φb }} {{ φc }} {{ φr }})) (at level 20).
 
 (* MARK: control flow terminals *)
-Lemma tac_wp_break s E v φ:
-  (φ $ SBreak v) ⊢
-  WP (EBreak $ Val v) @ s; E {{ bot }} {{ φ }} {{ bot }} {{ bot }}.
+Lemma tac_wp_break v φ:
+  (φ v) ⊢
+  WP (EBreak $ Val v) {{ bot }} {{ φ }} {{ bot }} {{ bot }}.
 Proof.
   assert ((EBreak $ Val v) = (of_sval $ SBreak v)); auto.
   rewrite H.
@@ -56,9 +58,9 @@ Proof.
   auto.
 Qed.
 
-Lemma tac_wp_continue s E φ:
-  (φ SContinue) ⊢
-  WP (EContinue) @ s; E {{ bot }} {{ bot }} {{ φ }} {{ bot }}.
+Lemma tac_wp_continue φ:
+  (φ $ LitV LitUnit) ⊢
+  WP (EContinue) {{ bot }} {{ bot }} {{ φ }} {{ bot }}.
 Proof.
   assert (EContinue = (of_sval SContinue)); auto.
   rewrite H.
@@ -67,9 +69,9 @@ Proof.
   auto.
 Qed.
 
-Lemma tac_wp_return s E v φ:
-  (φ $ SReturn v) ⊢
-  WP (EReturn $ Val v) @ s; E {{ bot }} {{ bot }} {{ bot }} {{ φ }}.
+Lemma tac_wp_return v φ:
+  (φ v) ⊢
+  WP (EReturn $ Val v) {{ bot }} {{ bot }} {{ bot }} {{ φ }}.
 Proof.
   assert ((EReturn $ Val v) = (of_sval $ SReturn v)); auto.
   rewrite H.
@@ -77,5 +79,71 @@ Proof.
   rewrite wp_unfold /wp_pre to_of_val.
   auto.
 Qed.
+
+(* MARK: loop *)
+Lemma tac_wp_loop e I φb φr:
+  {{ I }} e {{ λ v, I }} {{ φb }} {{ λ v, I }} {{ φr }} ⊢
+  {{ I }} (loop e) {{ φb }} {{ bot }} {{ bot }} {{ φr }}.
+Proof.
+  iIntros "#Hbdy !# H".
+  destruct e.
+  - rewrite wp_unfold /wp_pre; simpl.
+    rewrite wp_unfold /wp_pre; simpl.
+    iIntros (σ1 κ κs _) "[Hs Hproph]".
+    (* iMod (inv_alloc ⊤ _ _ with "Hi") as "Hinv". *)
+    iApply fupd_frame_l.
+    iSplit.
+    + iPureIntro. unfold reducible. simpl.
+      exists nil, (LoopB v v), σ1, nil.
+      apply (Ectx_step _ _ _ _ _ _ EmptyCtx (LoopB v v) (LoopB v v)); auto.
+      apply LoopBS.
+    + iAssert emp%I as "Htmp"; auto.
+      iMod (inv_alloc ⊤ _ _ with "Htmp") as "Hinv"; iClear "Htmp".
+
+      iInv "Hinv" as "H1" "Hclose".
+
+      eassert (⊤ = ↑⊤). { auto. }
+      epose proof (difference_diag_L (↑⊤)).
+      rewrite <- H in H0 at 1.
+      (* FIXME: stuck here *)
+      rewrite <- H0.
+      unfold fupd.
+      rewrite H0.
+
+      Search (_ ∖ ↑_).
+      SearchAbout UpClose.
+      replace ∅ with (⊤ ∖ ↑⊤).
+      iModIntro.
+
+      rewrite difference_diag_L.
+      epose proof (non_empty_difference (↑⊤) ⊤).
+      eassert (↑⊤ ⊂ ⊤); 
+      Locate union_difference_L.
+      Search (_ ∖ _).
+      simpl.
+      replace (⊤ ∖ ↑⊤) with ⊤.
+      iModIntro. 
+    
+    iIntros (e2 σ2 efs).
+
+    unfold fupd. unfold bi_fupd_fupd.
+    simpl.
+    unfold uPred_fupd.
+    Search fupd.
+    unfold bi_fupd_fupd.
+
+    simpl. unfold uPred_fupd.
+
+    iModIntro.
+    
+    iFrame "H1 H2".
+    destruct s.
+    2:{ } 
+    + unfold reducible. 
+  iApply wp_bind.
+    
+  iPoseProof "Hinv I" as "H1".
+  
+
 
 End multi_post.
